\input{header.tex}

\setcounter{theorem}{2}
\begin{exercise}[BH.5.3] 
\begin{solution}
    \begin{enumerate}
        \item We have $g(x) \geq 0$ since both $F$ and $f$ are nonnegative. Making the substitution $u=F(x)$, so $d u=f(x) d x$, we have
        $$
        \int_{-\infty}^{\infty} g(x) d x=2 \int_{-\infty}^{\infty} F(x) f(x) d x=2 \int_0^1 u d u=1.
        $$
        \item  We have $h(x) \geq 0$ since $f$ is nonnegative. Then
        $$
        \int_{-\infty}^{\infty} h(x) d x=\frac{1}{2} \int_{-\infty}^{\infty} f(-x) d x+\frac{1}{2} \int_{-\infty}^{\infty} f(x) d x=\frac{1}{2}+\frac{1}{2}=1
        $$
        since
        $$
        \int_{-\infty}^{\infty} f(-x) d x=-\int_{\infty}^{-\infty} f(u) d u=\int_{-\infty}^{\infty} f(u) d u=1
        $$
    \end{enumerate}
\end{solution}
\end{exercise}

\input{trailer.tex}
