\input{header.tex}
\setcounter{theorem}{23}
\begin{exercise} BH.6.24
\begin{hint}
Use that $X-Y = X+(-Y)$, and then that the mgf of the sum of two independent rvs  is equal to the product of the mgfs. Then solve the integrals.

To solve the mgf of $L$, realize that the integral runs from $-\infty$ to $\infty$. Then split the integral into a part from $-\infty$ to 0, and a second from $0$ to $\infty$. Then solve each of the integrals and compare what you get from the mgf of $X+(-Y)$.
\end{hint}

\begin{solution}
Check out the hint.

I prefer to keep $\lambda$ general for the moment, because like this I can use pattern recognition during the computations.
\begin{align*}
  M_{X}(s) &= \int_0^{\infty} \lambda e^{sx} e^{-\lambda x}\d x = \frac{\lambda}{\lambda - s}\\
  M_{-Y}(s) &= \int_0^{\infty} \lambda e^{-sx} e^{-\lambda x}\d x = \frac{\lambda}{\lambda +s}\\
  M_{X-Y}(s) &= M_X(s) M_{-Y}(x) = \frac{\lambda^{2}}{(\lambda-s)(\lambda+s)} = \frac{\lambda^{2}}{\lambda^{2}-s^2}.
\end{align*}
Now fill in $\lambda=1$.

\begin{align*}
  M_L(s) &= \frac{1}{2}\int_{-\infty}^{\infty} e^{sx} e^{-|x|}\d x = \frac{1}{2} \int_{-\infty}^{0} e^{sx} e^{-|x|}\d x + \frac{1}{2} \int_{0}^{\infty} e^{sx} e^{-|x|}\d x  \\
 &= \frac{1}{2} \int_{0}^{\infty} e^{-sx} e^{-x}\d x + \frac{1}{2} \int_{0}^{\infty} e^{sx} e^{-x}\d x  = \frac{1}{2} \frac{1}{1+s} + \frac{1}{2}\frac{1}{1-s} = \\
&=\frac{1}{(1+s)(1-s)} = \frac{1}{1-s^{2}}.
\end{align*}

The  mgfs of $X-Y$, with $\lambda=1$, is the  same as the mgf of $L$, hence $X-Y$ has the Laplace distribution. Note that the mgfs are the same \emph{on an open, non-empty, interval} $s\in (-1, 1)$.
\end{solution}
\end{exercise}
\input{trailer.tex}
